Update Logic, Task, Theory

proofs/core/Theory.v
@@ -3,6 +3,15 @@ Require Export FullInterp.
 Set Bullet Behavior "Strict Subproofs".
 (*Why3 Theories*)
 
+(*TODO: move*)
+Definition add_map_elts {A B: Type} `{countable.Countable A} (m: amap A B) (l: list (A * B)) : amap A B :=
+  fold_right (fun x acc => amap_set acc (fst x) (snd x)) m l.
+
+(*TODO: move*)
+Definition amap_map_key_val {A B C D : Type} `{countable.Countable A} `{countable.Countable C} (f: A -> C) (g: B -> D)
+  (m: amap A B) : amap C D :=
+  add_map_elts amap_empty (map (fun x => (f (fst x), g (snd x))) (elements m)).
+
 
 (*We depart from Why3 notation slightly here, since we make a distinction
   between a context (with declarations) and a theory
@@ -41,36 +50,27 @@ Set Bullet Behavior "Strict Subproofs".
 
 Section Sub.
 
-Variable (tys: list (vty * vty))
-(funs: list (funsym * funsym)) (preds: list (predsym * predsym)).
+Variable (tys: amap vty vty)
+(funs: amap funsym funsym) (preds: amap predsym predsym).
 
-Variable tys_srts: forallb is_sort (map snd tys).
-Lemma tys_sorts: forall x, In x (map snd tys) -> type_vars x = nil.
+Variable tys_srts: forallb is_sort (vals tys).
+Lemma tys_sorts: forall x, In x (vals tys) -> aset_is_empty (type_vars x).
 Proof.
   unfold is_true in tys_srts.
   rewrite forallb_forall in tys_srts.
   auto.
-  intros. unfold is_sort in tys_srts.
-  specialize (tys_srts _ H).
-  rewrite fold_is_true in tys_srts.
-  rewrite null_nil in tys_srts. auto.
 Qed.
 
-Definition sub_from_map {A: Set} (eq_dec: forall (x y: A), {x=y} +{x<>y})
-  (m: list (A * A)) (x: A) :=
-  match (get_assoc_list eq_dec m x) with
-  | Some y => y
-  | None => x
-  end.
 
-Definition sub_tys := sub_from_map vty_eq_dec tys.
-Definition sub_funs := sub_from_map funsym_eq_dec funs.
-Definition sub_preds := sub_from_map predsym_eq_dec preds.
+Definition sub_tys t := lookup_default tys t t.
+Definition sub_funs f := lookup_default funs f f.
+Definition sub_preds p := lookup_default preds p p.
+
 
 (*Sub in vty*)
 Fixpoint sub_in_vty (t: vty) :=
   (*Should make more efficient and only need 1 lookup*)
-  if in_dec vty_eq_dec t  (map fst tys) then 
+  if amap_mem t tys then 
   sub_tys t else
   match t with
   | vty_cons ts vs => vty_cons ts (map sub_in_vty vs)
@@ -78,18 +78,22 @@ Fixpoint sub_in_vty (t: vty) :=
   end.
 
 Lemma sub_tys_vars: forall x,
-  sublist (type_vars (sub_tys x)) (type_vars x).
+  asubset (type_vars (sub_tys x)) (type_vars x).
 Proof.
-  intros.
-  unfold sub_tys, sub_from_map.
-  destruct (get_assoc_list vty_eq_dec tys x) eqn : Ha;
-  [| apply sublist_refl].
-  apply get_assoc_list_some in Ha.
-  rewrite tys_sorts; [intros y [] | rewrite in_map_iff].
-  exists (x, v); auto.
+  intros x.
+  unfold sub_tys, lookup_default.
+  destruct (amap_lookup tys x) as [y|] eqn : Hlook.
+  - rewrite asubset_def. intros z Hmemz. unfold is_true in tys_srts.
+    rewrite forallb_forall in tys_srts.
+    specialize (tys_srts y).
+    forward tys_srts.
+    { rewrite in_vals_iff. exists x; auto. }
+    unfold is_sort in tys_srts.
+    exfalso. apply aset_is_empty_mem with (x:=z) in tys_srts. contradiction.
+  - apply asubset_refl.
 Qed.
 
-Lemma sub_tys_sort: forall x,
+(* Lemma sub_tys_sort: forall x,
   type_vars x = nil ->
   type_vars (sub_tys x) = nil.
 Proof.
@@ -98,20 +102,19 @@ Proof.
   - apply get_assoc_list_some in Ha.
     apply tys_sorts. rewrite in_map_iff. exists (x, v); auto.
   - auto.
-Qed.
+Qed. *)
 
 Lemma sub_in_vty_vars t:
-  sublist (type_vars (sub_in_vty t)) (type_vars t).
+  asubset (type_vars (sub_in_vty t)) (type_vars t).
 Proof.
   induction t; simpl; auto;
   match goal with
   | |- context [if ?b then ?c else ?d] => destruct b
-  end; simpl; try apply sublist_refl;
+  end; simpl; try apply asubset_refl;
   try apply sub_tys_vars.
-  clear n.
-  induction vs; simpl in *; try apply sublist_refl.
+  induction vs; simpl in *; try apply asubset_refl.
   inversion H; subst.
-  apply sublist_union; auto.
+  rewrite !aset_big_union_cons. apply asubset_union; auto.
 Qed.
 
 Lemma check_args_sub {params args}:
@@ -122,17 +125,18 @@ Proof.
   rewrite <- !(reflect_iff _ _ (check_args_correct _ _)); intros.
   rewrite in_map_iff in H0.
   destruct H0 as [t [Ht Hint]]; subst.
-  eapply sublist_trans.
+  eapply asubset_trans.
   apply sub_in_vty_vars. auto.
 Qed.
 
 Lemma check_sublist_sub {t params}:
-  check_sublist (type_vars t) params ->
-  check_sublist (type_vars (sub_in_vty t)) params.
+  check_asubset (type_vars t) params ->
+  check_asubset (type_vars (sub_in_vty t)) params.
 Proof.
-  unfold is_true.
-  rewrite <- !(reflect_iff _ _ (check_sublist_correct _ _)); intros.
-  eapply sublist_trans. apply sub_in_vty_vars. auto.
+  destruct (check_asubset _ _); [|discriminate]. intros _.
+  destruct (check_asubset _ _); auto. exfalso.
+  apply n.
+  eapply asubset_trans. apply sub_in_vty_vars. auto.
 Qed.
 
 (*Sub in fpsym*)
@@ -233,7 +237,7 @@ Definition is_ts_sub (ts: typesym) : bool :=
     match v with
     | vty_cons ts' _ => typesym_eq_dec ts ts'
     | _ => false
-    end) (map fst tys).
+    end) (keylist tys).
 
 Definition sub_ctx_map (c: context)  :
   context :=
@@ -242,9 +246,9 @@ Definition sub_ctx_map (c: context)  :
     (*Abstract: remove iff instantiate*)
     | abs_type ts => if is_ts_sub ts then acc
       else x :: acc
-    | abs_fun f => if in_dec funsym_eq_dec f (map fst funs) then acc
+    | abs_fun f => if amap_mem f funs then acc
       else x :: acc
-    | abs_pred p => if in_dec predsym_eq_dec p (map fst preds) then acc
+    | abs_pred p => if amap_mem p preds  then acc
       else x :: acc
     (*Concrete - need to substitute*)
     | datatype_def m =>  
@@ -267,25 +271,25 @@ End Sub.
 (*From why3 theory.ml - they use string -> typesym, etc maps
   I should too, eventually*)
 Record namespace := mk_ns {
-  ns_ts: list (string * typesym);
-  ns_fs: list (string * funsym);
-  ns_ps: list (string * predsym)
+  ns_ts: amap string typesym;
+  ns_fs: amap string funsym;
+  ns_ps: amap string predsym
 }.
 
 Definition ts_in_ns (t: typesym) (n: namespace) : bool :=
-  match (get_assoc_list string_dec (ns_ts n) (ts_name t) ) with
+  match (amap_lookup (ns_ts n) (ts_name t)) with
   | Some t1 => typesym_eq_dec t t1
   | None => false
   end.
 
 Definition fs_in_ns (f: funsym) (n: namespace) : bool :=
-  match (get_assoc_list string_dec (ns_fs n) (s_name f) ) with
+  match (amap_lookup (ns_fs n) (s_name f) ) with
   | Some f1 => funsym_eq_dec f f1
   | None => false
   end.
 
 Definition ps_in_ns (p: predsym) (n: namespace) : bool :=
-  match (get_assoc_list string_dec (ns_ps n) (s_name p) ) with
+  match (amap_lookup (ns_ps n) (s_name p) ) with
   | Some p1 => predsym_eq_dec p p1
   | None => false
   end.
@@ -321,6 +325,7 @@ Proof.
   induction t; simpl; auto.
   induction vs; simpl; auto.
   inversion H; subst.
+  rewrite !aset_big_union_cons.
   rewrite H2. f_equal. auto.
 Qed.
 
@@ -334,13 +339,13 @@ Proof.
   intros.
   rewrite in_map_iff in H0.
   destruct H0 as [t [Ht Hint]]; subst.
-  rewrite qual_vty_vars in H1.
+  rewrite qual_vty_vars.
   apply (H _ Hint); auto.
 Qed.
 
 Lemma check_sublist_qual {t params}:
-  check_sublist (type_vars t) params ->
-  check_sublist (type_vars (qual_vty t)) params.
+  check_asubset (type_vars t) params ->
+  check_asubset (type_vars (qual_vty t)) params.
 Proof.
   rewrite qual_vty_vars; auto.
 Qed.
@@ -456,10 +461,10 @@ End QualNames.
   we do not implement that for the moment.
 *)
 
-Definition ty_map : Set := {l: list (vty * vty) |
-  forallb is_sort (map snd l)}.
+Definition ty_map : Type := {l: amap vty vty |
+  forallb is_sort (vals l)}.
 
-Inductive tdecl : Set :=
+Inductive tdecl : Type :=
   | tdef : def -> tdecl
   | tprop : prop_kind -> string -> formula -> tdecl
   (*Use a theory (copy all of its definitions).
@@ -468,7 +473,7 @@ Inductive tdecl : Set :=
   (*Clone a theory - instantiating some parameters and giving
     a qualified name*)
   | tclone: list tdecl -> option string -> ty_map ->
-    list (funsym * funsym) -> list (predsym * predsym) -> tdecl.
+    amap funsym funsym -> amap predsym predsym -> tdecl.
 
 Definition theory := list tdecl.
 
@@ -496,34 +501,33 @@ From Equations Require Import Equations.
   (*We need a bunch of utilities*)
 (*Utilities for namespace (move)*)
 Definition emp_namespace : namespace :=
-  mk_ns nil nil nil.
+  mk_ns amap_empty amap_empty amap_empty.
 
 Definition add_ts_to_ns (tss: list typesym) (n: namespace) : namespace :=
-  mk_ns (map (fun x => (ts_name x, x)) tss ++ (ns_ts n)) (ns_fs n) (ns_ps n).
+  mk_ns (add_map_elts (ns_ts n) (map (fun x => (ts_name x, x)) tss)) (ns_fs n) (ns_ps n).
 
 Definition add_fs_to_ns (fss: list funsym) (n: namespace) : namespace :=
-  mk_ns (ns_ts n) (map (fun (x: funsym) => (s_name x, x)) fss ++ (ns_fs n))
+  mk_ns (ns_ts n) (add_map_elts (ns_fs n) (map (fun (x: funsym) => (s_name x, x)) fss))
     (ns_ps n).
 
 Definition add_ps_to_ns (pss: list predsym) (n: namespace) : namespace :=
   mk_ns (ns_ts n) (ns_fs n) 
-  (map (fun (x: predsym) => (s_name x, x)) pss ++ (ns_ps n)).
+  (add_map_elts (ns_ps n) (map (fun (x: predsym) => (s_name x, x)) pss)).
 
 Definition add_def_to_ns (d: def) (n: namespace) : namespace :=
   add_ps_to_ns (predsyms_of_def d) 
     (add_fs_to_ns (funsyms_of_def d)
       (add_ts_to_ns (typesyms_of_def d) n)).
 
-(*Note: should really be union*)
 Definition merge_ns (n1 n2: namespace) : namespace :=
-  mk_ns ((ns_ts n1) ++ (ns_ts n2)) ((ns_fs n1) ++ (ns_fs n2))
-    ((ns_ps n1) ++ (ns_ps n2)).
+  mk_ns (aunion (ns_ts n1) (ns_ts n2)) (aunion (ns_fs n1) (ns_fs n2))
+    (aunion (ns_ps n1) (ns_ps n2)).
 
 (*Add s as prefix to all entries in namespace*)
 Definition qualify_all (s: string) (n: namespace) : namespace :=
-  mk_ns (map (fun x => (add_prefix s (fst x), qual_ts_n s n (snd x))) (ns_ts n))
-    (map (fun x => (add_prefix s (fst x), qual_funsym_n s n (snd x))) (ns_fs n))
-    (map (fun x => (add_prefix s (fst x), qual_predsym_n s n (snd x))) (ns_ps n)).
+  mk_ns (amap_map_key_val (fun s1 => add_prefix s s1) (fun s2 =>qual_ts_n s n s2) (ns_ts n))
+    (amap_map_key_val (fun s1 => add_prefix s s1) (fun s2 =>qual_funsym_n s n s2) (ns_fs n))
+    (amap_map_key_val (fun s1 => add_prefix s s1) (fun s2 =>qual_predsym_n s n s2) (ns_ps n)).
 
 
 (*Get all exported names (only) from a theory*)
@@ -775,22 +779,23 @@ Definition tyconst_def (n: string) : def :=
 
 (*Get the type variables, substitute each with a fresh type constant*)
 Definition mk_mono (names: list string) (f: formula) : formula :=
-  if null (fmla_type_vars f) then f else
-  ty_subst_wf_fmla (fmla_type_vars f) (map tyconst names) f.
+  if aset_is_empty (fmla_type_vars f) then f else
+  ty_subst_wf_fmla (aset_to_list (fmla_type_vars f)) (map tyconst names) f.
 
 Lemma mk_mono_mono (names: list string) f:
-  length names = length (fmla_type_vars f) ->
+  length names = aset_size (fmla_type_vars f) ->
   closed_formula f ->
   mono (mk_mono names f).
 Proof.
   intros.
   unfold mono, mk_mono.
-  destruct (null (fmla_type_vars f)) eqn : Hvars; auto.
+  destruct (aset_is_empty (fmla_type_vars f)) eqn : Hvars; auto.
   apply ty_subst_srts_vars_f.
   - intros ty. rewrite in_map_iff. intros [n [Hty Hinn]]; subst.
     reflexivity.
   - intros x.
     rewrite make_fmla_wf_type_vars; auto.
+    simpl_set. auto.
 Qed.
 
 End Mono.
@@ -815,7 +820,7 @@ Fixpoint valid_theory (t: theory) : Prop :=
     | _ =>
       valid_theory tl /\
       (*If the formula is already monomorphic, dont do anything*)
-      (if null (fmla_type_vars f) then
+      (if aset_is_empty (fmla_type_vars f) then
       task_valid_closed (mk_task (theory_ctx_int tl) (theory_axioms_int tl)
       f) else
       (*Use exists so that the user can choose good names*)
